

From Eq. 1

$$\begin{aligned} \mathcal{L} = & -\frac{\beta^2}{2} Q_{23B} + g_1^2 \gamma_H^2 \beta^2 (2Q_{\phi,2} - 4Q_{\phi,1}) \\ & - \beta^2 \gamma_H 2 Q_{43B} \end{aligned} \quad \left[ \begin{array}{l} \text{following the} \\ \text{conv. from Wells} \end{array} \right]$$

Matching in the Warsaw basis:

$$c_{23B} = -\beta^2/2$$

$$c_{\phi,1} = -2 g_1^2 \gamma_H^2 \beta^2 = -\frac{1}{2} g_1^2 \beta^2$$

$$c_{43B} = -2 \beta^2 \gamma_H = -\beta^2$$

Oblique params: [Table 7 from Wells]

$$\begin{aligned} \hat{S} &= g_2^2 \left[ \frac{1}{4} c_{43B} - \frac{1}{2} c_{23B} + \dots \right] \\ & \quad \quad \quad \text{not generated} \\ &= \frac{1}{2} g_2^2 \left[ \frac{1}{2} (-\beta^2) - (-\beta^2/2) \right] \\ &= \frac{1}{2} g_2^2 \left[ -\beta^2/2 + \beta^2/2 \right] = 0 \end{aligned}$$

$$\begin{aligned} T &= -\frac{1}{2} c_{\phi,1} + g_1^2 \frac{1}{2} (c_{43B} - c_{23B}) \\ &= -\frac{1}{2} \left( -\frac{1}{2} g_1^2 \beta^2 \right) + g_1^2 \frac{1}{2} \left( -\beta^2 - (-\beta^2/2) \right) \\ &= \frac{1}{4} g_1^2 \beta^2 - \frac{1}{4} g_1^2 \beta^2 = 0 \end{aligned}$$

$$\begin{aligned} Y &= -g_2^2 \frac{1}{2} c_{23B} \\ &= -g_2^2 \frac{1}{2} \left( -\beta^2/2 \right) = g_2^2 \beta^2/4 \end{aligned}$$

In our basis, from Eq. 19 the matching reads

$$c_{23B} = -\beta^2/2$$

$$c_{\phi,1} = 2 g_1^2 \gamma_H^2 \beta^2 = \frac{1}{2} g_1^2 \beta^2$$

$$c_{BW} = -\frac{1}{2} g_1 g_2 \beta^2 \gamma_H = -\frac{1}{4} g_1 g_2 \beta^2$$

...

From our paper,

$$\begin{aligned} S &= g_2/g_1 c_{BW} - g_2^2 \frac{1}{2} c_{23B} + \dots \\ &= g_2 \left[ \frac{1}{g_1} \left( -\frac{1}{4} g_1 g_2 \beta^2 \right) - g_2 \frac{1}{2} \left( -\beta^2/2 \right) \right] \\ &= g_2 \left[ -\frac{1}{4} g_2 \beta^2 + \frac{1}{4} g_2 \beta^2 \right] = 0 \checkmark \end{aligned}$$

$$\begin{aligned} T &= -\frac{1}{2} \left[ c_{\phi,1} + g_1^2 c_{23B} \right] + \dots \\ &= -\frac{1}{2} \left[ \frac{1}{2} g_1^2 \beta^2 + g_1^2 \left( -\beta^2/2 \right) \right] \\ &= 0 \checkmark \end{aligned}$$

$$\begin{aligned} Y &= -g_2^2 \frac{1}{2} c_{23B} = -g_2^2 \frac{1}{2} \left( -\beta^2/2 \right) \\ &= g_2^2 \frac{1}{4} \beta^2 \checkmark \end{aligned}$$